src/test/dafny/MemoryVerif.dfy
@@ -65,18 +65,18 @@ abstract module MemoryVerif_01 {
   {
     //  address is in range, no expansion 
     if vm.Peek(0) as nat + 31 < vm.MemSize() {
-      var r := Bytecode.MStore(Gas.GasBerlin(MSTORE, vm)); 
+      var r := Bytecode.MStore(Gas.GasBerlin(MSTORE, vm));
       assert r.Gas() == vm.Gas() - Gas.G_VERYLOW;
     } 
    
     // memory is empty, address required is 0, Expansion should be 32 bytes
-    if vm.Peek(0) == 0 && vm.MemSize() == 0 && vm.Gas() >= 200 {
+    if vm.Peek(0) == 0 && vm.MemSize() == 0 && vm.Gas() >= 200 { 
         assert vm.Peek(0) as nat + 31 >= vm.MemSize();
         //  compute expanded size
         var ex := Memory.SmallestLarg32(vm.Peek(0) as nat + 31);
         //  expansion is 32 bytes
         assert ex == 32;
-        var exCost := Gas.computeDynGasMSTORE(vm.evm.memory, vm.Peek(0) as nat);
+        var exCost := Gas.ComputeDynGasMSTORE(vm.evm.memory, vm.Peek(0) as nat);
         assert exCost == Gas.G_MEMORY * 32 + 2; 
 
         var r := Bytecode.MStore(Gas.GasBerlin(MSTORE, vm));
